src/SSA.v
@@ -4538,105 +4538,6 @@ Section SSAStoreEq.
       repeat split_disjoint
     end.
 
-  Definition bvs_eqi (E : SSATE.env) (s1 s2 : SSAStore.t) :=
-    forall x, SSATE.mem x E -> SSAStore.acc x s1 = SSAStore.acc x s2.
-
-  Lemma bvs_eqi_refl E s : bvs_eqi E s s.
-  Proof. move=> *; reflexivity. Qed.
-
-  Lemma bvs_eqi_sym E s1 s2 : bvs_eqi E s1 s2 -> bvs_eqi E s2 s1.
-  Proof. move=> Heqi x Hx. exact: (Logic.eq_sym (Heqi x Hx)). Qed.
-
-  Lemma bvs_eqi_trans E s1 s2 s3 :
-    bvs_eqi E s1 s2 -> bvs_eqi E s2 s3 -> bvs_eqi E s1 s3.
-  Proof.
-    move=> H12 H23 x Hx. rewrite (H12 x Hx) (H23 x Hx). reflexivity.
-  Qed.
-
-  Lemma bvs_eqi_submap E1 E2 s1 s2 :
-    TELemmas.submap E1 E2 -> bvs_eqi E2 s1 s2 -> bvs_eqi E1 s1 s2.
-  Proof.
-    move=> Hsubm Heqi x Hx. exact: (Heqi x (TELemmas.submap_mem Hsubm Hx)).
-  Qed.
-
-  Lemma bvs_eqi_conform E s1 s2 :
-    bvs_eqi E s1 s2 -> SSAStore.conform s1 E -> SSAStore.conform s2 E.
-  Proof.
-    move=> Heqi Hco x Hmem. rewrite (Hco x Hmem). rewrite (Heqi x Hmem).
-    reflexivity.
-  Qed.
-
-  Lemma bvs_eqi_acc2z E s1 s2 x :
-    bvs_eqi E s1 s2 -> SSATE.mem x E -> acc2z E x s1 = acc2z E x s2.
-  Proof.
-    move=> Heqi Hmem. rewrite /acc2z. rewrite (Heqi x Hmem). reflexivity.
-  Qed.
-
-  Lemma bvs_eqi_eval_eexp E e s1 s2 :
-    are_defined (vars_eexp e) E -> bvs_eqi E s1 s2 ->
-    eval_eexp e E s1 = eval_eexp e E s2.
-  Proof.
-    elim: e => //=.
-    - move=> v Hdef Heqi. rewrite are_defined_singleton in Hdef.
-      move/memdefP: Hdef => Hmem. exact: (bvs_eqi_acc2z Heqi Hmem).
-    - move=> op e IH Hdef Heqi. rewrite (IH Hdef Heqi). reflexivity.
-    - move=> op e1 IH1 e2 IH2 Hdef Heqi. rewrite are_defined_union in Hdef.
-      move/andP: Hdef => [Hdef1 Hdef2].
-      rewrite (IH1 Hdef1 Heqi) (IH2 Hdef2 Heqi). reflexivity.
-  Qed.
-
-  Lemma bvs_eqi_eval_ebexp E e s1 s2 :
-    are_defined (vars_ebexp e) E -> bvs_eqi E s1 s2 ->
-    eval_ebexp e E s1 <-> eval_ebexp e E s2.
-  Proof.
-    elim: e => //=.
-    - move=> e1 e2 Hdef Heqi. rewrite are_defined_union in Hdef.
-      move/andP: Hdef => [Hdef1 Hdef2].
-      rewrite (bvs_eqi_eval_eexp Hdef1 Heqi) (bvs_eqi_eval_eexp Hdef2 Heqi). done.
-    - move=> e1 e2 e3 Hdef Heqi. repeat rewrite are_defined_union in Hdef.
-      move/andP: Hdef => [Hdef1 /andP [Hdef2 Hdef3]].
-      rewrite (bvs_eqi_eval_eexp Hdef1 Heqi) (bvs_eqi_eval_eexp Hdef2 Heqi)
-              (bvs_eqi_eval_eexp Hdef3 Heqi). done.
-    - move=> e1 IH1 e2 IH2 Hdef Heqi. rewrite are_defined_union in Hdef.
-      move/andP: Hdef => [Hdef1 Hdef2]. move: (IH1 Hdef1 Heqi) (IH2 Hdef2 Heqi).
-      tauto.
-  Qed.
-
-  Lemma bvs_eqi_eval_rexp E e s1 s2 :
-    are_defined (vars_rexp e) E -> bvs_eqi E s1 s2 ->
-    eval_rexp e s1 = eval_rexp e s2.
-  Proof.
-    elim: e => //=.
-    - move=> x Hdef Heqi. rewrite are_defined_singleton in Hdef.
-      move/memdefP: Hdef => Hmem. exact: (Heqi x Hmem).
-    - move=> _ op e IH Hdef Heqi. rewrite (IH Hdef Heqi). reflexivity.
-    - move=> _ op e1 IH1 e2 IH2 Hdef Heqi. rewrite are_defined_union in Hdef.
-      move/andP: Hdef => [Hdef1 Hdef2]. rewrite (IH1 Hdef1 Heqi) (IH2 Hdef2 Heqi).
-      reflexivity.
-    - move=> _ e IH n Hdef Heqi. rewrite (IH Hdef Heqi). reflexivity.
-    - move=> _ e IH n Hdef Heqi. rewrite (IH Hdef Heqi). reflexivity.
-  Qed.
-
-  Lemma bvs_eqi_eval_rbexp E e s1 s2 :
-    are_defined (vars_rbexp e) E -> bvs_eqi E s1 s2 ->
-    eval_rbexp e s1 <-> eval_rbexp e s2.
-  Proof.
-    elim: e => //=.
-    - move=> _ e1 e2 Hdef Heqi. rewrite are_defined_union in Hdef.
-      move/andP: Hdef => [Hdef1 Hdef2].
-      rewrite (bvs_eqi_eval_rexp Hdef1 Heqi) (bvs_eqi_eval_rexp Hdef2 Heqi). done.
-    - move=> _ op e1 e2 Hdef Heqi. rewrite are_defined_union in Hdef.
-      move/andP: Hdef => [Hdef1 Hdef2].
-      rewrite (bvs_eqi_eval_rexp Hdef1 Heqi) (bvs_eqi_eval_rexp Hdef2 Heqi). done.
-    - move=> e IH Hdef Heqi. move: (IH Hdef Heqi). tauto.
-    - move=> e1 IH1 e2 IH2 Hdef Heqi. rewrite are_defined_union in Hdef.
-      move/andP: Hdef => [Hdef1 Hdef2]. move: (IH1 Hdef1 Heqi) (IH2 Hdef2 Heqi).
-      tauto.
-    - move=> e1 IH1 e2 IH2 Hdef Heqi. rewrite are_defined_union in Hdef.
-      move/andP: Hdef => [Hdef1 Hdef2]. move: (IH1 Hdef1 Heqi) (IH2 Hdef2 Heqi).
-      tauto.
-  Qed.
-
   Ltac intro_neqs :=
     match goal with
     | H : is_true (SSATE.mem ?x ?E) |- _ =>
@@ -4678,6 +4579,17 @@ Section SSAStoreEq.
     (case: i => /=);
       try (move=> *; ssa_vars_unchanged_instr_to_mem;
                   invert_eval_instr; by decide_eqi).
+  Qed.
+
+  Lemma bvs_eqi_eval_rng_instr E i s1 s2 :
+    ssa_vars_unchanged_instr (vars_env E) i ->
+    eval_instr E (rng_instr i) s1 s2 ->
+    bvs_eqi E s1 s2.
+  Proof.
+    (case: i => /=);
+      try (move=> *; ssa_vars_unchanged_instr_to_mem;
+                  invert_eval_instr; by decide_eqi).
+    case => e r /=. move=> Hun Hei. inversion_clear Hei. exact: bvs_eqi_refl.
   Qed.
 
   Lemma bvs_eqi_eval_program E p s1 s2 :
